ReverseAddNext.fst
@@ -1295,3 +1295,356 @@ let local_profile_witness_92502871604050616929528 () : Lemma (
   reverse_add_18408442064004592449047_to_92502871604050616929528 ();
   no_overflow_outer_sum_6_to_9_implies_next_witness next5_source;
   ()
+
+let next6_source : numeral 10 = next5_target
+
+let next6_reversed : numeral 10 =
+  [9; 2; 5; 0; 2; 8; 7; 1; 6; 0; 4; 0; 5; 0; 6; 1; 6; 9; 2; 9; 5; 2; 8]
+
+let next6_target : numeral 10 =
+  [7; 5; 0; 0; 5; 7; 4; 3; 2; 1; 9; 0; 9; 0; 2; 3; 3; 8; 5; 9; 0; 5; 7; 1]
+
+let reverse_list_next6_source () : Lemma (rev next6_source == next6_reversed) =
+  assert (rev [9] == [9]);
+  rev_cons 2 [9];
+  rev_cons 5 [2; 9];
+  rev_cons 9 [5; 2; 9];
+  rev_cons 0 [9; 5; 2; 9];
+  rev_cons 2 [0; 9; 5; 2; 9];
+  rev_cons 8 [2; 0; 9; 5; 2; 9];
+  rev_cons 4 [8; 2; 0; 9; 5; 2; 9];
+  rev_cons 0 [4; 8; 2; 0; 9; 5; 2; 9];
+  rev_cons 6 [0; 4; 8; 2; 0; 9; 5; 2; 9];
+  rev_cons 1 [6; 0; 4; 8; 2; 0; 9; 5; 2; 9];
+  rev_cons 6 [1; 6; 0; 4; 8; 2; 0; 9; 5; 2; 9];
+  rev_cons 0 [6; 1; 6; 0; 4; 8; 2; 0; 9; 5; 2; 9];
+  rev_cons 5 [0; 6; 1; 6; 0; 4; 8; 2; 0; 9; 5; 2; 9];
+  rev_cons 0 [5; 0; 6; 1; 6; 0; 4; 8; 2; 0; 9; 5; 2; 9];
+  rev_cons 4 [0; 5; 0; 6; 1; 6; 0; 4; 8; 2; 0; 9; 5; 2; 9];
+  rev_cons 0 [4; 0; 5; 0; 6; 1; 6; 0; 4; 8; 2; 0; 9; 5; 2; 9];
+  rev_cons 6 [0; 4; 0; 5; 0; 6; 1; 6; 0; 4; 8; 2; 0; 9; 5; 2; 9];
+  rev_cons 1 [6; 0; 4; 0; 5; 0; 6; 1; 6; 0; 4; 8; 2; 0; 9; 5; 2; 9];
+  rev_cons 7 [1; 6; 0; 4; 0; 5; 0; 6; 1; 6; 0; 4; 8; 2; 0; 9; 5; 2; 9];
+  rev_cons 8 [7; 1; 6; 0; 4; 0; 5; 0; 6; 1; 6; 0; 4; 8; 2; 0; 9; 5; 2; 9];
+  rev_cons 2 [8; 7; 1; 6; 0; 4; 0; 5; 0; 6; 1; 6; 0; 4; 8; 2; 0; 9; 5; 2; 9];
+  rev_cons 5 [2; 8; 7; 1; 6; 0; 4; 0; 5; 0; 6; 1; 6; 0; 4; 8; 2; 0; 9; 5; 2; 9];
+  rev_cons 2 [5; 2; 8; 7; 1; 6; 0; 4; 0; 5; 0; 6; 1; 6; 0; 4; 8; 2; 0; 9; 5; 2; 9];
+  rev_cons 9 [2; 5; 2; 8; 7; 1; 6; 0; 4; 0; 5; 0; 6; 1; 6; 0; 4; 8; 2; 0; 9; 5; 2; 9];
+  ()
+
+let value_next6_reversed () : Lemma (
+    value next6_reversed == 82592961605040617820529) =
+  value_cons #10 9 [2; 5; 0; 2; 8; 7; 1; 6; 0; 4; 0; 5; 0; 6; 1; 6; 9; 2; 9; 5; 2; 8];
+  value_cons #10 2 [5; 0; 2; 8; 7; 1; 6; 0; 4; 0; 5; 0; 6; 1; 6; 9; 2; 9; 5; 2; 8];
+  value_cons #10 5 [0; 2; 8; 7; 1; 6; 0; 4; 0; 5; 0; 6; 1; 6; 9; 2; 9; 5; 2; 8];
+  value_cons #10 0 [2; 8; 7; 1; 6; 0; 4; 0; 5; 0; 6; 1; 6; 9; 2; 9; 5; 2; 8];
+  value_cons #10 2 [8; 7; 1; 6; 0; 4; 0; 5; 0; 6; 1; 6; 9; 2; 9; 5; 2; 8];
+  value_cons #10 8 [7; 1; 6; 0; 4; 0; 5; 0; 6; 1; 6; 9; 2; 9; 5; 2; 8];
+  value_cons #10 7 [1; 6; 0; 4; 0; 5; 0; 6; 1; 6; 9; 2; 9; 5; 2; 8];
+  value_cons #10 1 [6; 0; 4; 0; 5; 0; 6; 1; 6; 9; 2; 9; 5; 2; 8];
+  value_cons #10 6 [0; 4; 0; 5; 0; 6; 1; 6; 9; 2; 9; 5; 2; 8];
+  value_cons #10 0 [4; 0; 5; 0; 6; 1; 6; 9; 2; 9; 5; 2; 8];
+  value_cons #10 4 [0; 5; 0; 6; 1; 6; 9; 2; 9; 5; 2; 8];
+  value_cons #10 0 [5; 0; 6; 1; 6; 9; 2; 9; 5; 2; 8];
+  value_cons #10 5 [0; 6; 1; 6; 9; 2; 9; 5; 2; 8];
+  value_cons #10 0 [6; 1; 6; 9; 2; 9; 5; 2; 8];
+  value_cons #10 6 [1; 6; 9; 2; 9; 5; 2; 8];
+  value_cons #10 1 [6; 9; 2; 9; 5; 2; 8];
+  value_cons #10 6 [9; 2; 9; 5; 2; 8];
+  value_cons #10 9 [2; 9; 5; 2; 8];
+  value_cons #10 2 [9; 5; 2; 8];
+  value_cons #10 9 [5; 2; 8];
+  value_cons #10 5 [2; 8];
+  value_cons #10 2 [8];
+  value_cons #10 8 [];
+  ()
+
+let value_next6_target () : Lemma (
+    value next6_target == 175095833209091234750057) =
+  value_cons #10 7 [5; 0; 0; 5; 7; 4; 3; 2; 1; 9; 0; 9; 0; 2; 3; 3; 8; 5; 9; 0; 5; 7; 1];
+  value_cons #10 5 [0; 0; 5; 7; 4; 3; 2; 1; 9; 0; 9; 0; 2; 3; 3; 8; 5; 9; 0; 5; 7; 1];
+  value_cons #10 0 [0; 5; 7; 4; 3; 2; 1; 9; 0; 9; 0; 2; 3; 3; 8; 5; 9; 0; 5; 7; 1];
+  value_cons #10 0 [5; 7; 4; 3; 2; 1; 9; 0; 9; 0; 2; 3; 3; 8; 5; 9; 0; 5; 7; 1];
+  value_cons #10 5 [7; 4; 3; 2; 1; 9; 0; 9; 0; 2; 3; 3; 8; 5; 9; 0; 5; 7; 1];
+  value_cons #10 7 [4; 3; 2; 1; 9; 0; 9; 0; 2; 3; 3; 8; 5; 9; 0; 5; 7; 1];
+  value_cons #10 4 [3; 2; 1; 9; 0; 9; 0; 2; 3; 3; 8; 5; 9; 0; 5; 7; 1];
+  value_cons #10 3 [2; 1; 9; 0; 9; 0; 2; 3; 3; 8; 5; 9; 0; 5; 7; 1];
+  value_cons #10 2 [1; 9; 0; 9; 0; 2; 3; 3; 8; 5; 9; 0; 5; 7; 1];
+  value_cons #10 1 [9; 0; 9; 0; 2; 3; 3; 8; 5; 9; 0; 5; 7; 1];
+  value_cons #10 9 [0; 9; 0; 2; 3; 3; 8; 5; 9; 0; 5; 7; 1];
+  value_cons #10 0 [9; 0; 2; 3; 3; 8; 5; 9; 0; 5; 7; 1];
+  value_cons #10 9 [0; 2; 3; 3; 8; 5; 9; 0; 5; 7; 1];
+  value_cons #10 0 [2; 3; 3; 8; 5; 9; 0; 5; 7; 1];
+  value_cons #10 2 [3; 3; 8; 5; 9; 0; 5; 7; 1];
+  value_cons #10 3 [3; 8; 5; 9; 0; 5; 7; 1];
+  value_cons #10 3 [8; 5; 9; 0; 5; 7; 1];
+  value_cons #10 8 [5; 9; 0; 5; 7; 1];
+  value_cons #10 5 [9; 0; 5; 7; 1];
+  value_cons #10 9 [0; 5; 7; 1];
+  value_cons #10 0 [5; 7; 1];
+  value_cons #10 5 [7; 1];
+  value_cons #10 7 [1];
+  value_cons #10 1 [];
+  ()
+
+let canonical_next6_reversed () : Lemma (canonical #10 next6_reversed) =
+  assert (canonical #10 [8]);
+  canonical_cons #10 2 [8];
+  canonical_cons #10 5 [2; 8];
+  canonical_cons #10 9 [5; 2; 8];
+  canonical_cons #10 0 [9; 5; 2; 8];
+  canonical_cons #10 2 [0; 9; 5; 2; 8];
+  canonical_cons #10 9 [2; 0; 9; 5; 2; 8];
+  canonical_cons #10 4 [9; 2; 0; 9; 5; 2; 8];
+  canonical_cons #10 0 [4; 9; 2; 0; 9; 5; 2; 8];
+  canonical_cons #10 6 [0; 4; 9; 2; 0; 9; 5; 2; 8];
+  canonical_cons #10 1 [6; 0; 4; 9; 2; 0; 9; 5; 2; 8];
+  canonical_cons #10 6 [1; 6; 0; 4; 9; 2; 0; 9; 5; 2; 8];
+  canonical_cons #10 0 [6; 1; 6; 0; 4; 9; 2; 0; 9; 5; 2; 8];
+  canonical_cons #10 5 [0; 6; 1; 6; 0; 4; 9; 2; 0; 9; 5; 2; 8];
+  canonical_cons #10 0 [5; 0; 6; 1; 6; 0; 4; 9; 2; 0; 9; 5; 2; 8];
+  canonical_cons #10 4 [0; 5; 0; 6; 1; 6; 0; 4; 9; 2; 0; 9; 5; 2; 8];
+  canonical_cons #10 0 [4; 0; 5; 0; 6; 1; 6; 0; 4; 9; 2; 0; 9; 5; 2; 8];
+  canonical_cons #10 6 [0; 4; 0; 5; 0; 6; 1; 6; 0; 4; 9; 2; 0; 9; 5; 2; 8];
+  canonical_cons #10 1 [6; 0; 4; 0; 5; 0; 6; 1; 6; 0; 4; 9; 2; 0; 9; 5; 2; 8];
+  canonical_cons #10 6 [1; 6; 0; 4; 0; 5; 0; 6; 1; 6; 0; 4; 9; 2; 0; 9; 5; 2; 8];
+  canonical_cons #10 9 [6; 1; 6; 0; 4; 0; 5; 0; 6; 1; 6; 0; 4; 9; 2; 0; 9; 5; 2; 8];
+  canonical_cons #10 2 [9; 6; 1; 6; 0; 4; 0; 5; 0; 6; 1; 6; 0; 4; 9; 2; 0; 9; 5; 2; 8];
+  canonical_cons #10 5 [2; 9; 6; 1; 6; 0; 4; 0; 5; 0; 6; 1; 6; 0; 4; 9; 2; 0; 9; 5; 2; 8];
+  canonical_cons #10 2 [5; 2; 9; 6; 1; 6; 0; 4; 0; 5; 0; 6; 1; 6; 0; 4; 9; 2; 0; 9; 5; 2; 8];
+  ()
+
+let canonical_next6_target () : Lemma (canonical #10 next6_target) =
+  assert (canonical #10 [1]);
+  canonical_cons #10 7 [1];
+  canonical_cons #10 5 [7; 1];
+  canonical_cons #10 0 [5; 7; 1];
+  canonical_cons #10 9 [0; 5; 7; 1];
+  canonical_cons #10 5 [9; 0; 5; 7; 1];
+  canonical_cons #10 8 [5; 9; 0; 5; 7; 1];
+  canonical_cons #10 3 [8; 5; 9; 0; 5; 7; 1];
+  canonical_cons #10 3 [3; 8; 5; 9; 0; 5; 7; 1];
+  canonical_cons #10 2 [3; 3; 8; 5; 9; 0; 5; 7; 1];
+  canonical_cons #10 0 [2; 3; 3; 8; 5; 9; 0; 5; 7; 1];
+  canonical_cons #10 9 [0; 2; 3; 3; 8; 5; 9; 0; 5; 7; 1];
+  canonical_cons #10 1 [9; 0; 2; 3; 3; 8; 5; 9; 0; 5; 7; 1];
+  canonical_cons #10 2 [1; 9; 0; 2; 3; 3; 8; 5; 9; 0; 5; 7; 1];
+  canonical_cons #10 4 [2; 1; 9; 0; 2; 3; 3; 8; 5; 9; 0; 5; 7; 1];
+  canonical_cons #10 0 [4; 2; 1; 9; 0; 2; 3; 3; 8; 5; 9; 0; 5; 7; 1];
+  canonical_cons #10 9 [0; 4; 2; 1; 9; 0; 2; 3; 3; 8; 5; 9; 0; 5; 7; 1];
+  canonical_cons #10 7 [9; 0; 4; 2; 1; 9; 0; 2; 3; 3; 8; 5; 9; 0; 5; 7; 1];
+  canonical_cons #10 5 [7; 9; 0; 4; 2; 1; 9; 0; 2; 3; 3; 8; 5; 9; 0; 5; 7; 1];
+  canonical_cons #10 0 [5; 7; 9; 0; 4; 2; 1; 9; 0; 2; 3; 3; 8; 5; 9; 0; 5; 7; 1];
+  canonical_cons #10 5 [0; 5; 7; 9; 0; 4; 2; 1; 9; 0; 2; 3; 3; 8; 5; 9; 0; 5; 7; 1];
+  canonical_cons #10 7 [5; 0; 5; 7; 9; 0; 4; 2; 1; 9; 0; 2; 3; 3; 8; 5; 9; 0; 5; 7; 1];
+  canonical_cons #10 5 [7; 5; 0; 5; 7; 9; 0; 4; 2; 1; 9; 0; 2; 3; 3; 8; 5; 9; 0; 5; 7; 1];
+  canonical_cons #10 7 [5; 7; 5; 0; 5; 7; 9; 0; 4; 2; 1; 9; 0; 2; 3; 3; 8; 5; 9; 0; 5; 7; 1];
+  ()
+
+let reverse_digits_next6_source () : Lemma (
+    reverse_digits #10 next6_source == next6_reversed) =
+  ReverseAddNext.canonical_next5_target ();
+  reverse_list_next6_source ();
+  value_next6_reversed ();
+  canonical_next6_reversed ();
+  reverse_digits_canonical #10 next6_source;
+  normalize_value #10 (rev next6_source);
+  assert (value (reverse_digits #10 next6_source) ==
+    82592961605040617820529);
+  digits_of_nat_of_canonical #10 (reverse_digits #10 next6_source);
+  digits_of_nat_of_canonical #10 next6_reversed;
+  assert (reverse_digits #10 next6_source == next6_reversed);
+  ()
+
+let reverse_add_92502871604050616929528_to_175095833209091234750057 () : Lemma (
+    reverse_add #10 next6_source == next6_target) =
+  ReverseAddNext.canonical_next5_target ();
+  reverse_add_value #10 next6_source;
+  ReverseAddNext.value_next5_target ();
+  reverse_digits_next6_source ();
+  value_next6_reversed ();
+  value_next6_target ();
+  assert (value (reverse_add #10 next6_source) ==
+    175095833209091234750057);
+  reverse_add_canonical #10 next6_source;
+  digits_of_nat_of_canonical #10 (reverse_add #10 next6_source);
+  canonical_next6_target ();
+  digits_of_nat_of_canonical #10 next6_target;
+  assert (reverse_add #10 next6_source == next6_target);
+  ()
+
+let trace_digits_profile_92502871604050616929528 () : Lemma (
+    trace_digits next6_source == next6_target) =
+  reverse_add_92502871604050616929528_to_175095833209091234750057 ();
+  trace_digits_equals_reverse_add next6_source;
+  assert (trace_digits next6_source == next6_target);
+  ()
+
+let trace_carries_next6_source () : Lemma (trace_carries next6_source ==
+    [0; 1; 0; 1; 1; 0; 1; 1; 0; 1; 0; 0; 0; 0; 0; 1; 0; 1; 1; 0; 0; 1; 0; 1]) =
+  reverse_list_next6_source ();
+  assert (trace_carries next6_source ==
+    (add_trace #10 next6_source next6_reversed 0).carries);
+  add_trace_carries_step #10 8 9
+    [2; 5; 9; 2; 9; 6; 1; 6; 0; 5; 0; 4; 0; 6; 1; 7; 8; 2; 0; 5; 2; 9]
+    [2; 5; 0; 2; 8; 7; 1; 6; 0; 4; 0; 5; 0; 6; 1; 6; 9; 2; 9; 5; 2; 8] 0;
+  add_trace_carries_step #10 2 2
+    [5; 9; 2; 9; 6; 1; 6; 0; 5; 0; 4; 0; 6; 1; 7; 8; 2; 0; 5; 2; 9]
+    [5; 0; 2; 8; 7; 1; 6; 0; 4; 0; 5; 0; 6; 1; 6; 9; 2; 9; 5; 2; 8] 1;
+  add_trace_carries_step #10 5 5
+    [9; 2; 9; 6; 1; 6; 0; 5; 0; 4; 0; 6; 1; 7; 8; 2; 0; 5; 2; 9]
+    [0; 2; 8; 7; 1; 6; 0; 4; 0; 5; 0; 6; 1; 6; 9; 2; 9; 5; 2; 8] 0;
+  add_trace_carries_step #10 9 0
+    [2; 9; 6; 1; 6; 0; 5; 0; 4; 0; 6; 1; 7; 8; 2; 0; 5; 2; 9]
+    [2; 8; 7; 1; 6; 0; 4; 0; 5; 0; 6; 1; 6; 9; 2; 9; 5; 2; 8] 1;
+  add_trace_carries_step #10 2 2
+    [9; 6; 1; 6; 0; 5; 0; 4; 0; 6; 1; 7; 8; 2; 0; 5; 2; 9]
+    [8; 7; 1; 6; 0; 4; 0; 5; 0; 6; 1; 6; 9; 2; 9; 5; 2; 8] 1;
+  add_trace_carries_step #10 9 8
+    [6; 1; 6; 0; 5; 0; 4; 0; 6; 1; 7; 8; 2; 0; 5; 2; 9]
+    [7; 1; 6; 0; 4; 0; 5; 0; 6; 1; 6; 9; 2; 9; 5; 2; 8] 0;
+  add_trace_carries_step #10 6 7
+    [1; 6; 0; 5; 0; 4; 0; 6; 1; 7; 8; 2; 0; 5; 2; 9]
+    [1; 6; 0; 4; 0; 5; 0; 6; 1; 6; 9; 2; 9; 5; 2; 8] 1;
+  add_trace_carries_step #10 1 1
+    [6; 0; 5; 0; 4; 0; 6; 1; 7; 8; 2; 0; 5; 2; 9]
+    [6; 0; 4; 0; 5; 0; 6; 1; 6; 9; 2; 9; 5; 2; 8] 1;
+  add_trace_carries_step #10 6 6
+    [0; 5; 0; 4; 0; 6; 1; 7; 8; 2; 0; 5; 2; 9]
+    [0; 4; 0; 5; 0; 6; 1; 6; 9; 2; 9; 5; 2; 8] 0;
+  add_trace_carries_step #10 0 0
+    [5; 0; 4; 0; 6; 1; 7; 8; 2; 0; 5; 2; 9]
+    [4; 0; 5; 0; 6; 1; 6; 9; 2; 9; 5; 2; 8] 1;
+  add_trace_carries_step #10 5 4
+    [0; 4; 0; 6; 1; 7; 8; 2; 0; 5; 2; 9]
+    [0; 5; 0; 6; 1; 6; 9; 2; 9; 5; 2; 8] 0;
+  add_trace_carries_step #10 0 0
+    [4; 0; 6; 1; 7; 8; 2; 0; 5; 2; 9]
+    [5; 0; 6; 1; 6; 9; 2; 9; 5; 2; 8] 0;
+  add_trace_carries_step #10 4 5
+    [0; 6; 1; 7; 8; 2; 0; 5; 2; 9]
+    [0; 6; 1; 6; 9; 2; 9; 5; 2; 8] 0;
+  add_trace_carries_step #10 0 0
+    [6; 1; 7; 8; 2; 0; 5; 2; 9]
+    [6; 1; 6; 9; 2; 9; 5; 2; 8] 0;
+  add_trace_carries_step #10 6 6
+    [1; 7; 8; 2; 0; 5; 2; 9]
+    [1; 6; 9; 2; 9; 5; 2; 8] 0;
+  add_trace_carries_step #10 1 1
+    [7; 8; 2; 0; 5; 2; 9]
+    [6; 9; 2; 9; 5; 2; 8] 1;
+  add_trace_carries_step #10 7 6
+    [8; 2; 0; 5; 2; 9]
+    [9; 2; 9; 5; 2; 8] 0;
+  add_trace_carries_step #10 8 9
+    [2; 0; 5; 2; 9]
+    [2; 9; 5; 2; 8] 1;
+  add_trace_carries_step #10 2 2
+    [0; 5; 2; 9]
+    [9; 5; 2; 8] 1;
+  add_trace_carries_step #10 0 9
+    [5; 2; 9]
+    [5; 2; 8] 0;
+  add_trace_carries_step #10 5 5
+    [2; 9]
+    [2; 8] 0;
+  add_trace_carries_step #10 2 2
+    [9]
+    [8] 1;
+  add_trace_carries_step #10 9 8 [] [] 0;
+  assert ((add_trace #10 [] [] 1).carries == [1]);
+  assert ((add_trace #10 next6_source next6_reversed 0).carries ==
+    [0; 1; 0; 1; 1; 0; 1; 1; 0; 1; 0; 0; 0; 0; 0; 1; 0; 1; 1; 0; 0; 1; 0; 1]);
+  ()
+
+let trace_profile_shape_92502871604050616929528 () : Lemma (
+    length (trace_digits next6_source) == length next6_source + 1) =
+  trace_digits_profile_92502871604050616929528 ();
+  length_of_eq #(digit 10) (trace_digits next6_source) next6_target;
+  assert (length next6_target == length next6_source + 1);
+  ()
+
+let trace_profile_final_carry_92502871604050616929528 () : Lemma (
+    nth (trace_carries next6_source) (length next6_source) == Some 1) =
+  trace_profile_shape_92502871604050616929528 ();
+  ReverseAddContinuation.final_carry_from_overflow_length next6_source;
+  ()
+
+let trace_profile_sums_92502871604050616929528 () : Lemma (
+    trace_sum_at next6_source 0 == 17 /\
+    trace_sum_at next6_source 1 == 4 /\
+    trace_sum_at next6_source 22 == 17) =
+  reverse_list_next6_source ();
+  ()
+
+let trace_profile_carry_facts_92502871604050616929528 () : Lemma (
+    trace_carry_at next6_source 1 == 1 /\
+    trace_carry_at next6_source 22 == 0 /\
+    trace_carry_at next6_source 2 == 0 /\
+    trace_carry_at next6_source 23 == 1) =
+  trace_carries_next6_source ();
+  ()
+
+let overflow_precondition_175095833209091234750057 () : Lemma (
+    canonical #10 next6_source /\
+    next6_source <> [] /\
+    length (trace_digits next6_source) == length next6_source + 1 /\
+    nth (trace_carries next6_source) (length next6_source) == Some 1 /\
+    1 <= trace_sum_at next6_source 0 /\
+    trace_sum_at next6_source 0 <= 18 /\
+    trace_sum_at next6_source 0 <> 10 /\
+    exists (i:nat). 0 < i /\ i < length next6_source /\
+      trace_sum_at next6_source i +
+          trace_sum_at next6_source (length next6_source - i) +
+          trace_carry_at next6_source i +
+          trace_carry_at next6_source (length next6_source - i) >=
+        10 + 10 *
+          (trace_carry_at next6_source (i + 1) +
+           trace_carry_at next6_source (length next6_source - i + 1))) =
+  ReverseAddNext.canonical_next5_target ();
+  assert (canonical #10 next6_source);
+  assert (next6_source <> []);
+  trace_profile_shape_92502871604050616929528 ();
+  trace_profile_final_carry_92502871604050616929528 ();
+  trace_profile_sums_92502871604050616929528 ();
+  trace_profile_carry_facts_92502871604050616929528 ();
+  assert (length (trace_digits next6_source) == length next6_source + 1);
+  assert (nth (trace_carries next6_source)
+    (length next6_source) == Some 1);
+  assert (trace_sum_at next6_source 0 == 17);
+  assert (trace_sum_at next6_source 1 == 4);
+  assert (trace_sum_at next6_source 22 == 17);
+  assert (trace_carry_at next6_source 1 == 1);
+  assert (trace_carry_at next6_source 22 == 0);
+  assert (trace_carry_at next6_source 2 == 0);
+  assert (trace_carry_at next6_source 23 == 1);
+  assert (1 <= trace_sum_at next6_source 0 /\
+    trace_sum_at next6_source 0 <= 18);
+  assert (trace_sum_at next6_source 0 <> 10);
+  let n : nat = length next6_source in
+  assert (0 < 1 /\ 1 < n);
+  assert (trace_sum_at next6_source 1 +
+      trace_sum_at next6_source (n - 1) +
+      trace_carry_at next6_source 1 +
+      trace_carry_at next6_source (n - 1) >=
+    10 + 10 *
+      (trace_carry_at next6_source 2 +
+       trace_carry_at next6_source (n - 1 + 1)));
+  exists_intro
+    (fun (i:nat) -> 0 < i /\ i < n /\
+      trace_sum_at next6_source i +
+          trace_sum_at next6_source (n - i) +
+          trace_carry_at next6_source i +
+          trace_carry_at next6_source (n - i) >=
+        10 + 10 *
+          (trace_carry_at next6_source (i + 1) +
+           trace_carry_at next6_source (n - i + 1)))
+    1;
+  ()
+
+let local_profile_witness_175095833209091234750057 () : Lemma (
+    trace_local_profile_complement_witness next6_target) =
+  overflow_precondition_175095833209091234750057 ();
+  reverse_add_92502871604050616929528_to_175095833209091234750057 ();
+  overflow_internal_cell_implies_next_witness next6_source;
+  ()
